Wavelet/Compile.lean
@@ -2,3 +2,5 @@ import Wavelet.Compile.Fn
 import Wavelet.Compile.Prog
 import Wavelet.Compile.MapChans
 import Wavelet.Compile.AffineOp
+import Wavelet.Compile.AffineVar
+import Wavelet.Compile.AffineChan
