Wavelet/Compile/AffineChan.lean
@@ -1,0 +1,44 @@
+import Wavelet.Dataflow
+
+namespace Wavelet.Dataflow
+
+open Semantics
+
+def AtomicProc.inputs [Arity Op] : AtomicProc Op χ V → List χ
+  | .op _ inputs _ => inputs.toList
+  | .switch _ inputs _ _ => inputs.toList
+  | .steer _ _ inputs _ => inputs.toList
+  | .carry _ _ inputs₁ inputs₂ _ => (inputs₁ ++ inputs₂).toList
+  | .merge _ inputs₁ inputs₂ _ => (inputs₁ ++ inputs₂).toList
+  | .forward inputs _ => inputs.toList
+  | .fork input _ => [input]
+  | .const _ act _ => [act]
+  | .forwardc inputs _ _ => inputs.toList
+  | .sink inputs => inputs.toList
+
+def AtomicProc.outputs [Arity Op] : AtomicProc Op χ V → List χ
+  | .op _ _ outputs => outputs.toList
+  | .switch _ _ outputs₁ outputs₂ => (outputs₁ ++ outputs₂).toList
+  | .steer _ _ _ outputs => outputs.toList
+  | .carry _ _ _ _ outputs => outputs.toList
+  | .merge _ _ _ outputs => outputs.toList
+  | .forward _ outputs => outputs.toList
+  | .fork _ outputs => outputs.toList
+  | .const _ _ outputs => outputs.toList
+  | .forwardc _ _ outputs => outputs.toList
+  | .sink _ => []
+
+/-- Each channel name is used at most once. -/
+def AtomicProcs.AffineChan [Arity Op] (aps : AtomicProcs Op χ V) : Prop
+  :=
+  (∀ (i : Fin aps.length),
+    aps[i].inputs.Nodup ∧ aps[i].outputs.Nodup) ∧
+  (∀ (i j : Fin aps.length), i ≠ j →
+    aps[i].inputs.Disjoint aps[j].inputs ∧
+    aps[i].outputs.Disjoint aps[j].outputs)
+
+/-- Each channel name is used at most once. -/
+def Proc.AffineChan [Arity Op] (proc : Proc Op χ V m n) : Prop
+  := proc.atoms.AffineChan
+
+end Wavelet.Dataflow
